Make more progress on labs exist cheat

compiler/backend/proofs/lab_to_targetProofScript.sml
@@ -259,6 +259,8 @@ val line_similar_def = Define `
   (line_similar (LabAsm a w bytes l) (LabAsm a' w' bytes' l') <=> (a = a')) /\
   (line_similar _ _ <=> F)`
 
+val line_similar_ind = theorem"line_similar_ind";
+
 val code_similar_def = Define `
   (code_similar [] [] = T) /\
   (code_similar ((Section s1 lines1)::rest1) ((Section s2 lines2)::rest2) <=>
@@ -3522,6 +3524,8 @@ val line_labs_exist_def = Define`
     ∀n1 n2. (n1,n2) ∈ labs_of a ⇒ lab_lookup n1 n2 labs ≠ NONE) ∧
   (line_labs_exist _ _ ⇔ T)`;
 
+val line_labs_exist_ind = theorem "line_labs_exist_ind";
+
 val _ = export_rewrites["labs_of_def","line_labs_exist_def"];
 
 val sec_labs_exist_def = Define`
@@ -3532,25 +3536,21 @@ val _ = overload_on("all_labs_exist",``λlabs code. EVERY (sec_labs_exist labs) 
 
 (* labs_exist preservation *)
 
-val labs_exist_add_nop = Q.store_thm("labs_exist_add_nop[simp]",
-  `∀nop aux.
-   EVERY (line_labs_exist labs) (add_nop nop aux) ⇔
-   EVERY (line_labs_exist labs) aux`,
-  recInduct add_nop_ind
-  \\ rw[add_nop_def]);
+val line_similar_line_labs_exist = Q.store_thm("line_similar_line_labs_exist",
+  `∀l1 l2. line_similar l1 l2 ⇒ (line_labs_exist labs l1 ⇔ line_labs_exist labs l2)`,
+  recInduct line_similar_ind
+  \\ rw[line_similar_def]);
 
-val labs_exist_pad_section = Q.store_thm("labs_exist_pad_section",
-  `∀nop ls acc.
-   EVERY (line_labs_exist labs) (pad_section nop ls acc) ⇔
-   EVERY (line_labs_exist labs) ls ∧ EVERY (line_labs_exist labs) acc`,
-  recInduct pad_section_ind
-  \\ rw[pad_section_def, EVERY_REVERSE]
-  \\ rw[EQ_IMP_THM] \\ fs[]);
+val code_similar_all_labs_exist = Q.store_thm("code_similar_all_labs_exist",
+  `∀c1 c2. code_similar c1 c2 ⇒ (all_labs_exist labs c1 ⇔ all_labs_exist labs c2)`,
+  recInduct code_similar_ind
+  \\ rw[code_similar_def]
+  \\ fs[LIST_REL_EL_EQN, EVERY_MEM, MEM_EL]
+  \\ metis_tac[line_similar_line_labs_exist]);
 
 val all_labs_exist_pad_code = Q.store_thm("all_labs_exist_pad_code[simp]",
   `∀nop code. all_labs_exist labs (pad_code nop code) ⇔ all_labs_exist labs code`,
-  recInduct pad_code_ind
-  \\ rw[pad_code_def, labs_exist_pad_section]);
+  metis_tac[code_similar_pad_code, code_similar_all_labs_exist, code_similar_refl]);
 
 val enc_lines_again_line_labs_exist = Q.store_thm("enc_lines_again_line_labs_exist",
   `∀labs ffis pos enc lines acc ok res ok' k.
@@ -3571,6 +3571,132 @@ val enc_secs_again_all_labs_exist = Q.store_thm("enc_secs_again_all_labs_exist",
   \\ rpt(pairarg_tac \\ fs[]) \\ rw[]
   \\ match_mp_tac enc_lines_again_line_labs_exist
   \\ asm_exists_tac \\ fs[]);
+
+val upd_lab_len_all_labs_exist = Q.store_thm("upd_lab_len_all_labs_exist",
+  `∀pos code. all_labs_exist labs (upd_lab_len pos code) ⇔ all_labs_exist labs code`,
+  metis_tac[code_similar_upd_lab_len, code_similar_all_labs_exist, code_similar_refl]);
+
+(* establishing labs_exist *)
+
+val line_get_code_labels_def = Define`
+  line_get_code_labels (Label _ l _) = {l} ∧
+  line_get_code_labels _ = {}`;
+val _ = export_rewrites["line_get_code_labels_def"];
+
+val sec_get_code_labels_def = Define`
+  sec_get_code_labels (Section n1 lines) =
+    (n1,0) INSERT
+    IMAGE (λn2. (n1,n2)) (BIGUNION (IMAGE line_get_code_labels (set lines)))`;
+
+val get_code_labels_def = Define`
+  get_code_labels code = BIGUNION (IMAGE sec_get_code_labels (set code))`;
+
+val get_code_labels_nil = Q.store_thm("get_code_labels_nil[simp]",
+  `get_code_labels [] = {}`, EVAL_TAC \\ rw[]);
+
+val get_code_labels_cons = Q.store_thm("get_code_labels_cons",
+  `get_code_labels (s::secs) = sec_get_code_labels s ∪ get_code_labels secs`,
+  rw[get_code_labels_def]);
+
+val line_similar_line_get_code_labels = Q.store_thm("line_similar_line_get_code_labels",
+  `∀l1 l2. line_similar l1 l2 ⇒ line_get_code_labels l1 = line_get_code_labels l2`,
+  recInduct line_similar_ind
+  \\ rw[line_similar_def]);
+
+val code_similar_get_code_labels = Q.store_thm("code_similar_get_code_labels",
+  `∀c1 c2. code_similar c1 c2 ⇒ get_code_labels c1 = get_code_labels c2`,
+  recInduct code_similar_ind
+  \\ rw[code_similar_def, get_code_labels_cons]
+  \\ AP_THM_TAC \\ AP_TERM_TAC
+  \\ rw[sec_get_code_labels_def]
+  \\ AP_TERM_TAC \\ AP_TERM_TAC \\ AP_TERM_TAC
+  \\ fs[Once EXTENSION,MEM_EL,LIST_REL_EL_EQN,PULL_EXISTS]
+  \\ metis_tac[line_similar_line_get_code_labels]);
+
+val line_get_labels_def = Define`
+  line_get_labels (LabAsm a _ _ _) = labs_of a ∧
+  line_get_labels _ = {}`;
+
+val sec_get_labels_def = Define`
+  sec_get_labels (Section _ lines) =
+    BIGUNION (IMAGE line_get_labels (set lines))`;
+
+val get_labels_def = Define`
+  get_labels code = BIGUNION (IMAGE sec_get_labels (set code))`;
+
+val labs_domain_def = Define`
+  labs_domain labs = { (n1, n2) | lab_lookup n1 n2 labs ≠ NONE }`;
+
+val labs_domain_insert = Q.store_thm("labs_domain_insert",
+  `k ∉ domain labs ⇒
+   labs_domain (insert k s labs) = IMAGE (λn2. (k,n2)) (domain s) ∪ labs_domain labs`,
+  rw[labs_domain_def,lab_lookup_def, lookup_insert, EXTENSION, EQ_IMP_THM]
+  \\ fs[case_eq_thms] \\ fs[domain_lookup]
+  \\ metis_tac[NOT_SOME_NONE,option_CASES]);
+
+val line_labs_exist_get_labels = Q.store_thm("line_labs_exist_get_labels",
+  `∀labs line. line_labs_exist labs line ⇔ line_get_labels line ⊆ labs_domain labs`,
+  recInduct line_labs_exist_ind
+  \\ rw[line_labs_exist_def, line_get_labels_def, labs_domain_def, SUBSET_DEF, FORALL_PROD]);
+
+val sec_labs_exist_get_labels = Q.store_thm("sec_labs_exist_get_labels",
+  `∀labs sec. sec_labs_exist labs sec ⇔ sec_get_labels sec ⊆ labs_domain labs`,
+  Cases_on`sec`
+  \\ rw[sec_labs_exist_def, sec_get_labels_def, line_labs_exist_get_labels,
+        EVERY_MEM, SUBSET_DEF, PULL_EXISTS]
+  \\ metis_tac[]);
+
+val all_labs_exist_get_labels = Q.store_thm("all_labs_exist_get_labels",
+  `all_labs_exist labs code ⇔ get_labels code ⊆ labs_domain labs`,
+  rw[EVERY_MEM, sec_labs_exist_get_labels, get_labels_def,
+     SUBSET_DEF, PULL_EXISTS]
+  \\ metis_tac[]);
+
+val line_similar_line_get_labels = Q.store_thm("line_similar_line_get_labels",
+  `∀l1 l2. line_similar l1 l2 ⇒ (line_get_labels l1 = line_get_labels l2)`,
+  recInduct line_similar_ind
+  \\ rw[line_similar_def, line_get_labels_def]);
+
+val code_similar_get_labels = Q.store_thm("code_similar_get_labels",
+  `∀c1 c2. code_similar c1 c2 ⇒ get_labels c1 = get_labels c2`,
+  recInduct code_similar_ind
+  \\ rw[code_similar_def, get_labels_def, sec_get_labels_def]
+  \\ AP_THM_TAC \\ AP_TERM_TAC \\ AP_TERM_TAC
+  \\ simp[Once EXTENSION, PULL_EXISTS]
+  \\ fs[LIST_REL_EL_EQN, MEM_EL]
+  \\ metis_tac[line_similar_line_get_labels]);
+
+val get_labels_upd_lab_len = Q.store_thm("get_labels_upd_lab_len[simp]",
+  `get_labels (upd_lab_len pos code) = get_labels code`,
+  metis_tac[code_similar_get_labels, code_similar_upd_lab_len, code_similar_refl]);
+
+val section_labels_line_get_code_labels = Q.store_thm("section_labels_line_get_code_labels",
+  `∀pos lines aux new_pos labs. section_labels pos lines aux = (new_pos, labs) ⇒
+   0 INSERT set (MAP FST labs) = 0 INSERT set (MAP FST aux) ∪ BIGUNION (IMAGE line_get_code_labels (set lines))`,
+  recInduct section_labels_ind
+  \\ rw[section_labels_def]
+  \\ rw[EXTENSION]
+  \\ metis_tac[]);
+
+val labs_domain_compute_labels_alt = Q.store_thm("labs_domain_compute_labels_alt",
+  `∀pos code labs.
+     ALL_DISTINCT (MAP Section_num code) ∧
+     DISJOINT (domain labs) (set (MAP Section_num code)) ⇒
+     labs_domain (compute_labels_alt pos code labs) =
+     get_code_labels code ∪ labs_domain labs`,
+  recInduct compute_labels_alt_ind
+  \\ rw[compute_labels_alt_def]
+  \\ pairarg_tac \\ fs[]
+  \\ fs[labs_domain_insert, domain_fromAList]
+  \\ simp[get_code_labels_cons]
+  \\ fs[sec_get_code_labels_def]
+  \\ imp_res_tac section_labels_line_get_code_labels
+  \\ fs[UNION_ASSOC]
+  \\ AP_THM_TAC \\ AP_TERM_TAC
+  \\ simp[UNION_COMM]
+  \\ AP_TERM_TAC
+  \\ fs[Once EXTENSION,PULL_EXISTS, FORALL_PROD]
+  \\ metis_tac[]);
 
 (* invariant: labels aligned at even positions *)
 
@@ -4330,7 +4456,24 @@ val remove_labels_loop_thm = Q.prove(
     \\ conj_tac >- (
       match_mp_tac enc_secs_again_all_labs_exist
       \\ asm_exists_tac \\ simp[]
-      \\ cheat (* need to prove all labs exist *))
+      \\ rw[all_labs_exist_get_labels]
+      \\ `MAP Section_num code2 = MAP Section_num code`
+      by metis_tac[code_similar_MAP_Section_num,
+                   enc_secs_again_IMP_similar,
+                   code_similar_upd_lab_len]
+      \\ qspecl_then[`init_pos`,`code2`,`init_labs`]mp_tac labs_domain_compute_labels_alt
+      \\ impl_tac >- metis_tac[]
+      \\ simp[] \\ disch_then kall_tac
+      \\ qspecl_then[`code2`,`code1`]mp_tac code_similar_get_code_labels
+      \\ impl_tac >- metis_tac[code_similar_upd_lab_len,code_similar_refl]
+      \\ rw[] \\ simp[Abbr`code2`]
+      \\ imp_res_tac enc_secs_again_IMP_similar
+      \\ drule code_similar_get_code_labels
+      \\ drule code_similar_get_labels
+      \\ disch_then(assume_tac o SYM)
+      \\ disch_then(assume_tac o SYM)
+      \\ rw[]
+      \\ cheat (* labels exist *))
     \\ match_mp_tac offset_ok_pad_code \\ fs[]
     \\ metis_tac[enc_secs_again_offset_ok])
   \\ conj_asm1_tac
